shift-reset/core/syntax_notation.v
@@ -4,18 +4,43 @@ Declare Scope term_scope.
 Delimit Scope term_scope with term.
 Bind Scope term_scope with term.
 
+Declare Custom Entry binder'.
+Declare Custom Entry exn_pattern.
 Declare Custom Entry term.
+Declare Custom Entry term1.
+Declare Custom Entry exn_term.
+
+Notation "'_'" := BAny (in custom binder' at level 0) : term_scope.
+Notation "x" := x (in custom binder' at level 0, x constr at level 0) : term_scope.
+
+Notation "'_'" := ExnPAny (in custom exn_pattern at level 0) : term_scope.
+Notation "x" := x (in custom exn_pattern at level 0, x constr at level 0) : term_scope.
+
+Notation "' ( tag x )" :=
+  (ExnPTag tag x) (in custom exn_pattern at level 10, tag custom exn_pattern, x custom exn_pattern) : term_scope.
 
 Notation "<{ t }>" := t (t custom term at level 99) : term_scope.
 Notation "( t )" := t (in custom term, t at level 99) : term_scope.
-Notation "t" := t (in custom term at level 0, t constr at level 0) : term_scope.
 Notation "{ t }" := t (in custom term, t constr) : term_scope.
+Notation "t" := t (in custom term at level 0, t constr at level 0) : term_scope.
+
+Notation "( t )" := t (in custom term1, t at level 99) : term_scope.
+Notation "( t )" := t (in custom exn_term, t at level 99) : term_scope.
+
+Notation "'fun' x => t" :=
+  (T1 x t)
+    (in custom term1 at level 69,
+        x custom binder' at level 0,
+        t custom term) : term_scope.
+
+Notation "'fun' x => t" :=
+  (ExnT x t)
+    (in custom exn_term at level 69,
+        x custom exn_pattern at level 10,
+        t custom term) : term_scope.
 
 Notation "a1 a2" :=
-  (TApp a1 a2)
-    (in custom term at level 10,
-        a1 custom term,
-        a2 custom term) : term_scope.
+  (TApp a1 a2) (in custom term at level 10, a1 custom term, a2 custom term) : term_scope.
 
 Notation "'if' a 'then' t1 'else' t2" :=
   (TIf a t1 t2)
@@ -27,7 +52,7 @@ Notation "'if' a 'then' t1 'else' t2" :=
 Notation "'let' x := t1 'in' t2" :=
   (TLet t1 (T1 x t2))
     (in custom term at level 69,
-        x at level 0,
+        x custom binder' at level 0,
         t1 custom term,
         t2 custom term,
         right associativity) : term_scope.
@@ -35,7 +60,9 @@ Notation "'let' x := t1 'in' t2" :=
 Notation "'let' f x1 .. xn := t1 'in' t2" :=
   (TLet (TFun (T1 x1 .. (TFun (T1 xn t1)) ..)) (T1 f t2))
     (in custom term at level 69,
-        f, x1, xn at level 0,
+        f custom binder' at level 0,
+        x1 custom binder' at level 0,
+        xn custom binder' at level 0,
         t1 custom term,
         t2 custom term,
         right associativity) : term_scope.
@@ -43,7 +70,8 @@ Notation "'let' f x1 .. xn := t1 'in' t2" :=
 Notation "'let' 'fix' f x := t1 'in' t2" :=
   (TLet (TFix (T2 f x t1)) (T1 f t2))
     (in custom term at level 69,
-        f, x at level 0,
+        f custom binder' at level 0,
+        x custom binder' at level 0,
         t1 custom term,
         t2 custom term,
         right associativity) : term_scope.
@@ -51,22 +79,19 @@ Notation "'let' 'fix' f x := t1 'in' t2" :=
 Notation "'let' 'fix' f x1 x2 .. xn := t1 'in' t2" :=
   (TLet (TFix (T2 f x1 (TFun (T1 x2 .. (TFun (T1 xn t1)) ..)))) (T1 f t2))
     (in custom term at level 69,
-        f, x1, x2, xn at level 0,
+        f custom binder' at level 0,
+        x1 custom binder' at level 0,
+        x2 custom binder' at level 0,
+        xn custom binder' at level 0,
         t1 custom term,
         t2 custom term,
         right associativity) : term_scope.
 
-Notation "'shift' k t" :=
-  (TShift (T1 k t))
-    (in custom term at level 69,
-        k at level 0,
-        t custom term at level 99) : term_scope.
+Notation "'shift' t" :=
+  (TShift t) (in custom term at level 69, t custom term1) : term_scope.
 
-Notation "'control' k t" :=
-  (TControl (T1 k t))
-    (in custom term at level 69,
-        k at level 0,
-        t custom term at level 99) : term_scope.
+Notation "'control' t" :=
+  (TControl t) (in custom term at level 69, t custom term1) : term_scope.
 
 Notation "'reset' t" :=
   (TReset t) (in custom term at level 69, t custom term) : term_scope.
@@ -77,26 +102,33 @@ Notation "'prompt' t" :=
 Notation "'fun' x1 .. xn => t" :=
   (TFun (T1 x1 .. (TFun (T1 xn t)) ..))
     (in custom term at level 69,
-        x1, xn at level 0,
+        x1 custom binder' at level 0,
+        xn custom binder' at level 0,
         t custom term at level 99) : term_scope.
 
 Notation "'fix' f x := t" :=
   (TFix (T2 f x t))
     (in custom term at level 69,
-        f, x at level 0,
+        f custom binder' at level 0,
+        x custom binder' at level 0,
         t custom term at level 99) : term_scope.
 
 Notation "'fix' f x1 x2 .. xn := t" :=
   (TFix (T2 f x1 (TFun (T1 x2 .. (TFun (T1 xn t)) ..))))
     (in custom term at level 69,
-        f, x1, x2, xn at level 0,
+        f custom binder' at level 0,
+        x1 custom binder' at level 0,
+        x2 custom binder' at level 0,
+        xn custom binder' at level 0,
         t custom term at level 99) : term_scope.
 
 Notation "()" := AUnit (in custom term at level 0) : term_scope.
-Notation "'_'" := BAny (in custom term at level 0) : term_scope.
 
 Notation "'not' a" :=
   (TPrim1 P1Not a) (in custom term at level 23, a custom term at level 0) : term_scope.
+
+Notation "- a" :=
+  (TPrim1 P1Neg a) (in custom term at level 23, a custom term at level 0) : term_scope.
 
 Notation "'ref' a" :=
   (TRef a) (in custom term at level 23, a custom term at level 0) : term_scope.
@@ -108,93 +140,52 @@ Notation "'free' a" :=
   (TFree a) (in custom term at level 23, a custom term at level 0) : term_scope.
 
 Notation "a1 + a2" :=
-  (TPrim2 P2Add a1 a2)
-    (in custom term at level 40,
-        a1 custom term,
-        a2 custom term) : term_scope.
+  (TPrim2 P2Add a1 a2) (in custom term at level 40, a1 custom term, a2 custom term) : term_scope.
 
 Notation "a1 - a2" :=
-  (TPrim2 P2Sub a1 a2)
-    (in custom term at level 40,
-        a1 custom term,
-        a2 custom term) : term_scope.
+  (TPrim2 P2Sub a1 a2) (in custom term at level 40, a1 custom term, a2 custom term) : term_scope.
 
 Notation "a1 * a2" :=
-  (TPrim2 P2Mul a1 a2)
-    (in custom term at level 39,
-        a1 custom term,
-        a2 custom term) : term_scope.
+  (TPrim2 P2Mul a1 a2) (in custom term at level 39, a1 custom term, a2 custom term) : term_scope.
 
 Notation "a1 = a2" :=
-  (TPrim2 P2Eq a1 a2)
-    (in custom term at level 50,
-        a1 custom term,
-        a2 custom term) : term_scope.
+  (TPrim2 P2Eq a1 a2) (in custom term at level 50, a1 custom term, a2 custom term) : term_scope.
 
 Notation "a1 <> a2" :=
-  (TPrim2 P2Eq a1 a2)
-    (in custom term at level 50,
-        a1 custom term,
-        a2 custom term) : term_scope.
+  (TPrim2 P2Neq a1 a2) (in custom term at level 50, a1 custom term, a2 custom term) : term_scope.
 
 Notation "a1 < a2" :=
-  (TPrim2 P2Lt a1 a2)
-    (in custom term at level 50,
-        a1 custom term,
-        a2 custom term) : term_scope.
+  (TPrim2 P2Lt a1 a2) (in custom term at level 50, a1 custom term, a2 custom term) : term_scope.
 
 Notation "a1 <= a2" :=
-  (TPrim2 P2Le a1 a2)
-    (in custom term at level 50,
-        a1 custom term,
-        a2 custom term) : term_scope.
+  (TPrim2 P2Le a1 a2) (in custom term at level 50, a1 custom term, a2 custom term) : term_scope.
 
 Notation "a1 > a2" :=
-  (TPrim2 P2Gt a1 a2)
-    (in custom term at level 50,
-        a1 custom term,
-        a2 custom term) : term_scope.
+  (TPrim2 P2Gt a1 a2) (in custom term at level 50, a1 custom term, a2 custom term) : term_scope.
 
 Notation "a1 >= a2" :=
-  (TPrim2 P2Ge a1 a2)
-    (in custom term at level 50,
-        a1 custom term,
-        a2 custom term) : term_scope.
+  (TPrim2 P2Ge a1 a2) (in custom term at level 50, a1 custom term, a2 custom term) : term_scope.
 
 Notation "a1 && a2" :=
-  (TPrim2 P2And a1 a2)
-    (in custom term at level 50,
-        a1 custom term,
-        a2 custom term) : term_scope.
+  (TPrim2 P2And a1 a2) (in custom term at level 50, a1 custom term, a2 custom term) : term_scope.
 
 Notation "a1 || a2" :=
-  (TPrim2 P2Or a1 a2)
-    (in custom term at level 50,
-        a1 custom term,
-        a2 custom term) : term_scope.
+  (TPrim2 P2Or a1 a2) (in custom term at level 50, a1 custom term, a2 custom term) : term_scope.
 
 Notation "a1 'xor' a2" :=
-  (TPrim2 P2And a1 a2)
-    (in custom term at level 50,
-        a1 custom term,
-        a2 custom term) : term_scope.
+  (TPrim2 P2Xor a1 a2) (in custom term at level 50, a1 custom term, a2 custom term) : term_scope.
 
 Notation "a1 <- a2" :=
-  (TSet a1 a2)
-    (in custom term at level 65,
-        a1 custom term,
-        a2 custom term) : term_scope.
+  (TSet a1 a2) (in custom term at level 65, a1 custom term, a2 custom term) : term_scope.
 
 Notation "a1 , a2" :=
-  (TPair a1 a2)
-    (in custom term at level 65,
-        a1 custom term,
-        a2 custom term) : term_scope.
+  (TPair a1 a2) (in custom term at level 65, a1 custom term, a2 custom term) : term_scope.
 
 Notation "'let' ( x1 , x2 ) := a 'in' t" :=
   (TSplit a (T2 x1 x2 t))
     (in custom term at level 69,
-        x1, x2 at level 0,
+        x1 custom binder' at level 0,
+        x2 custom binder' at level 0,
         a custom term,
         t custom term,
         right associativity) : term_scope.
@@ -202,7 +193,8 @@ Notation "'let' ( x1 , x2 ) := a 'in' t" :=
 Notation "'let' x1 , x2 := a 'in' t" :=
   (TSplit a (T2 x1 x2 t))
     (in custom term at level 69,
-        x1, x2 at level 0,
+        x1 custom binder' at level 0,
+        x2 custom binder' at level 0,
         a custom term,
         t custom term,
         right associativity) : term_scope.
@@ -217,15 +209,22 @@ Notation "'match' a 'with' | 'Inl' x1 => t1 | 'Inr' x2 => t2 'end'" :=
   (TCase a (T1 x1 t1) (T1 x2 t2))
     (in custom term at level 69,
         a custom term,
-        x1, x2 at level 0,
+        x1 custom binder' at level 0,
+        x2 custom binder' at level 0,
         t1 custom term,
         t2 custom term) : term_scope.
 
-Notation "'exception' x a" :=
-  (TExn x a)
+Notation "'exception' tag a" :=
+  (TExn tag a)
     (in custom term at level 23,
-        x at level 0,
+        tag at level 0,
         a custom term at level 0) : term_scope.
 
 Notation "'raise' a" :=
   (TRaise a) (in custom term at level 23, a custom term at level 0) : term_scope.
+
+Notation "'try' t1 ; t2" :=
+  (TTry t1 t2)
+    (in custom term at level 69,
+        t1 custom term,
+        t2 custom exn_term) : term_scope.
