shift-reset/core/tag.v
@@ -1,0 +1,6 @@
+From Stdlib Require Import String.
+
+Record tag : Type := Tag { tag_car : string }.
+
+Definition tag_eq_dec : forall (tag1 tag2 : tag), {tag1 = tag2} + {tag1 <> tag2}.
+Proof. decide equality; auto using string_dec. Defined.
